Try to simplify repeat_test

iodiv/TestTauIODiv.fst
@@ -128,13 +128,14 @@ let repeat_pure (t : unit -> unit) : IODiv unit (requires fun hist -> True) (ens
 let repeat_more (fd : file_descr) : IODiv unit (requires fun hist -> is_open fd hist) (ensures fun hist r -> diverges r)
 = repeat_with_inv #(fun hist -> is_open fd hist) #(fun tr -> True) (fun _ -> let s = read fd in ())
 
-let repeat_test (s : string) : IODiv unit (requires fun hist -> True) (ensures fun hist r -> exists fd. diverges r /\ repeat_inv_post (fun tr -> exists s. tr == [ERead fd s]) r)
-// by (explode () ; dump "bla")
-= admit () ;
+let repeat_test (s : string) : IODiv unit (requires fun hist -> True) (ensures fun hist r -> (*exists fd.*) diverges r (*/\ repeat_inv_post (fun tr -> exists s. tr == [ERead fd s]) r*))
+by (explode () ; bump_nth 12 ; smt ())
+= admit () ; // Subtyping fails but I don't understand why
   let fd = open_file s in
   repeat (fun b hist -> is_open fd hist) (fun tr -> exists s. tr == [ERead fd s]) (fun b ->
     let x = read fd in
-    if b && x = "" then true else false
+    // if b && x = "" then true else false
+    true
   ) false
 
 let test_using_assume (fd : file_descr) : IODiv string (requires fun _ -> True) (ensures fun hist r -> terminates r) =
